the blues are still blue

coq/two/IndistinguishabilityTwo.v
@@ -11,7 +11,7 @@ Context (L : two)
         (P : value -> value -> Prop)
         (Prefl : forall x, P x x).
 
-Fixpoint atom_Lequiv a1 a2 : Prop :=
+Fixpoint atom_LPequiv a1 a2 : Prop :=
   match a1, a2 with
     | Atom v1 l1, Atom v2 l2 =>
       (L = Bottom2 /\ l1 = l2 /\ l1 = Top2 /\
@@ -19,32 +19,32 @@ Fixpoint atom_Lequiv a1 a2 : Prop :=
          | VNat n1, VNat n2 => P v1 v2
          | _, _ => True
        end) \/
-      (L = Bottom2 /\ l1 = l2 /\ l1 = Bottom2 /\ value_Lequiv v1 v2) \/
-      (L = Top2 /\ l1 = l2 /\ value_Lequiv v1 v2)
+      (L = Bottom2 /\ l1 = l2 /\ l1 = Bottom2 /\ value_LPequiv v1 v2) \/
+      (L = Top2 /\ l1 = l2 /\ value_LPequiv v1 v2)
   end
-with value_Lequiv v1 v2 : Prop :=
+with value_LPequiv v1 v2 : Prop :=
        match v1, v2 with
          | VNat n1, VNat n2 => n1 = n2
          | VClos e1 t1, VClos e2 t2 =>
-           list_forall2 atom_Lequiv e1 e2 /\ term_equiv t1 t2
+           list_forall2 atom_LPequiv e1 e2 /\ term_equiv t1 t2
          | VNat _, _ | VClos _ _, _ => False
        end.
 
-Definition env_Lequiv : env -> env -> Prop :=
-  list_forall2 atom_Lequiv.
+Definition env_LPequiv : env -> env -> Prop :=
+  list_forall2 atom_LPequiv.
 
-Lemma atom_Lequiv_lab_inv :
+Lemma atom_LPequiv_lab_inv :
   forall v1 v2 l1 l2,
-    atom_Lequiv (Atom v1 l1) (Atom v2 l2) ->
+    atom_LPequiv (Atom v1 l1) (Atom v2 l2) ->
     l1 = l2.
 Proof.
   intros. inversion H; inversion H0; destruct_conjs; auto.
 Qed.
 
-Lemma atom_Lequiv_raise :
+Lemma atom_LPequiv_raise :
   forall v1 v2,
-    atom_Lequiv (Atom v1 Bottom2) (Atom v2 Bottom2) ->
-    atom_Lequiv (Atom v1 Top2) (Atom v2 Top2).
+    atom_LPequiv (Atom v1 Bottom2) (Atom v2 Bottom2) ->
+    atom_LPequiv (Atom v1 Top2) (Atom v2 Top2).
 Proof.
   intros v1 v2 H. destruct L.
     destruct v1; destruct v2; destruct H; destruct H; destruct_conjs;
@@ -62,3 +62,43 @@ Proof.
 Qed.
 
 End IndistinguishabilityTwo.
+
+Definition atom_Lequiv := fun L => atom_LPequiv L (fun _ _ => True).
+
+Definition value_Lequiv := fun L => value_LPequiv L (fun _ _ => True).
+
+Definition env_Lequiv := fun L => env_LPequiv L (fun _ _ => True).
+
+Lemma atom_value_env_LPequiv_Lequiv :
+  forall L P,
+    (forall a1 a2,
+       atom_LPequiv L P a1 a2 -> atom_Lequiv L a1 a2)
+    /\ (forall v1 v2,
+          value_LPequiv L P v1 v2 -> value_Lequiv L v1 v2)
+    /\ (forall e1 e2,
+          env_LPequiv L P e1 e2 -> env_Lequiv L e1 e2).
+Proof.
+  Admitted. (* TODO *)
+
+Lemma atom_LPequiv_Lequiv :
+  forall L P a1 a2,
+    atom_LPequiv L P a1 a2 -> atom_Lequiv L a1 a2.
+Proof. apply atom_value_env_LPequiv_Lequiv. Qed.
+
+Lemma value_LPequiv_Lequiv :
+  forall L P v1 v2,
+    value_LPequiv L P v1 v2 -> value_Lequiv L v1 v2.
+Proof. apply atom_value_env_LPequiv_Lequiv. Qed.
+
+Lemma env_LPequiv_Lequiv :
+  forall L P e1 e2,
+    env_LPequiv L P e1 e2 -> env_Lequiv L e1 e2.
+Proof. apply atom_value_env_LPequiv_Lequiv. Qed.
+
+Lemma atom_Lequiv_lab_inv :
+  forall L v1 v2 l1 l2,
+    atom_Lequiv L (Atom v1 l1) (Atom v2 l2) ->
+    l1 = l2.
+Proof.
+  intros. inversion H; inversion H0; destruct_conjs; auto.
+Qed.
