coq/two/LambdaTwoNI.v
@@ -34,11 +34,11 @@ Qed.
 Lemma NI_strong :
   forall pc1 pc2 e1 e2 t1 t2 a1 a2,
     pc1 = pc2 ->
-    env_Lequiv L P e1 e2 ->
+    env_LPequiv L P e1 e2 ->
     term_equiv t1 t2 ->
     pc1; e1 ⊢ t1 ⇓ a1 ->
     pc2; e2 ⊢ t2 ⇓ a2 ->
-    atom_Lequiv L P a1 a2.
+    atom_Lequiv L a1 a2.
 Proof.
   intros pc1 pc2 e1 e2 t1 t2 a1 a2 Hpc He Ht Heval.
   generalize dependent a2.
@@ -47,32 +47,35 @@ Proof.
   generalize dependent pc2.
   induction Heval;
     intros pc2 Hpc e2 He t2' Ht a3' Heval2'; destruct t2'; try inversion Ht.
-    (* Eval_nat *)
+  - (* Eval_nat *)
     inversion Heval2'. subst.
     destruct L; destruct pc2.
       right. left. auto.
       left. auto.
       right. right. auto.
       right. right. auto.
-    (* Eval_var *)
-    inversion Heval2'. subst. unfold env_Lequiv in He.
-    assert (atom_Lequiv L P (Atom v l) (Atom v0 l0)) by
+  - (* Eval_var *)
+    inversion Heval2'. subst. unfold env_LPequiv in He.
+    assert (atom_LPequiv L P (Atom v l) (Atom v0 l0)) by
         (eapply list_forall2_atIndex; eassumption).
     assert (l = l0) by
-        (eapply atom_Lequiv_lab_inv; eassumption).
+        (eapply atom_LPequiv_lab_inv; eassumption).
     subst.
     destruct pc2.
-      rewrite join_bot. assumption.
+      rewrite join_bot. eapply atom_LPequiv_Lequiv. eassumption.
       rewrite join_top. destruct l0.
-        apply atom_Lequiv_raise. apply Prefl. assumption. assumption.
-    (* Eval_lam *)
+        apply atom_LPequiv_raise in H0. eapply atom_LPequiv_Lequiv. eassumption.
+          assumption.
+        eapply atom_LPequiv_Lequiv. eassumption.
+  - (* Eval_lam *)
     inversion Heval2'. subst.
+    apply env_LPequiv_Lequiv in He.
     destruct L; destruct pc2.
-      right. left. auto.
+      right. left. auto. 
       left. auto.
       right. right. auto.
       right. right. auto.
-    (* Eval_app *)
+  - (* Eval_app *)
     inversion Heval2'. subst.
     rename l0 into l1'. rename a0 into a2'.
     assert (t2'1 = t1) by
@@ -80,45 +83,18 @@ Proof.
     assert (t2'2 = t2) by
         (apply term_equiv_eq; symmetry; auto).
     subst. clear H. clear H0. clear Ht.
-    remember (Atom (VClos e1' t1') l1) as f1.
-    remember (Atom (VClos e1'0 t1'0) l1') as f2.
-    assert (atom_Lequiv L P f1 f2) by
-        (eapply IHHeval1; eauto). subst.
-    assert (l1' = l1) by
-        (apply atom_Lequiv_lab_inv in H; auto). subst.
-    destruct L.
-      destruct l1.
-        destruct H; destruct H; destruct_conjs; try inversion H1; inversion H.
-          assert (atom_Lequiv Bottom2 P a2 a2').
-            apply IHHeval2 in H6; auto.
-          assert (env_Lequiv Bottom2 P e1' e1'0) by auto.
-          assert (env_Lequiv Bottom2 P (a2 :: e1') (a2' :: e1'0)).
-            split; auto. 
-          apply IHHeval3 in H8; auto.
-        destruct a3 as [v3 l3]; destruct v3; destruct l3;
-        destruct a3' as [v3' l3']; destruct v3'; destruct l3';
-          apply eval_pc_lower_bound in H8; inversion H8;
-          apply eval_pc_lower_bound in Heval3; inversion Heval3;
-          left; auto; repeat (split; auto).
-        admit. (* TODO: L=Bottom2 l1=Top2, need P (VNat n) (VNat n0) *)
-      assert (env_Lequiv Top2 P e1' e1'0) by
-            (destruct H; destruct H; destruct_conjs; inversion H; auto).
-      assert (atom_Lequiv Top2 P a2 a2') by
-            (apply IHHeval2 in H6; auto).
-      assert (env_Lequiv Top2 P (a2 :: e1') (a2' :: e1'0)) by
-          (split; auto).
-      assert (term_equiv t1' t1'0) by
-          (destruct H; destruct H; destruct_conjs; inversion H; auto).
-      apply IHHeval3 in H8; auto.
-Qed.
+    assert (l1' = l1).
+      apply IHHeval1 in H3. apply atom_Lequiv_lab_inv in H3.
+        symmetry. assumption. reflexivity. assumption. reflexivity. subst.
+    Admitted.
       
 (** * General non-interference theorem. *)
 Theorem general_non_interference :
   forall pc e1 e2 t a1 a2,
-    env_Lequiv L P e1 e2 ->
+    env_LPequiv L P e1 e2 ->
     pc; e1 ⊢ t ⇓ a1 ->
     pc; e2 ⊢ t ⇓ a2 ->
-    atom_Lequiv L P a1 a2.
+    atom_Lequiv L a1 a2.
 Proof. intros. eapply NI_strong; eauto. Qed.
 
 End NI.
